specs/lean/Synchronicity/TrieProgramTests.lean
@@ -33,6 +33,7 @@ private def run : List (Reply (Option ByteArray)) → Program Storage (Reply Loo
   | _ :: _, .request (.commit _) _ => none
   | _ :: _, .request (.rollback _) _ => none
   | _ :: _, .request (.readRows _ _ _ _ _ _) _ => none
+  | _ :: _, .request (.scanRows _ _ _ _ _ _) _ => none
   | _ :: _, .request (.upsert _ _ _ _ _) _ => none
   | _ :: _, .request (.deleteRows _ _ _ _) _ => none
   | _ :: _, .request (.readInput _ _ _) _ => none
